spec+proof: return new flag state after invokeSetFlags
This requires that the flags being set are first masked, to avoid
spurious flags that are not supported by the specific seL4 configuration
being used.

Signed-off-by: Corey Lewis <corey.lewis@proofcraft.systems>

spec/haskell/src/SEL4/Object/TCB.lhs
@@ -556,11 +556,16 @@ Modifying the current thread may require rescheduling because modified registers
 
 > invokeTCB (SetFlags tcb flagsClear flagsSet) =
 >   withoutPreemption $ do
+>     newFlags <- invokeSetFlags tcb flagsClear flagsSet
+>     return [newFlags]
+
+> invokeSetFlags :: PPtr TCB -> Word -> Word -> Kernel Word
+> invokeSetFlags tcb flagsClear flagsSet = do
 >     flags <- threadGet tcbFlags tcb
->     let newFlags = (flags .&. complement flagsClear) .|. flagsSet
+>     let newFlags = (flags .&. complement flagsClear) .|. (flagsSet .&. tcbFlagMask)
 >     setFlags tcb newFlags
 >     Arch.postSetFlags tcb newFlags
->     return []
+>     return newFlags
 
 \subsection{Decoding Domain Invocations}
 
