proof/refine/RISCV64/Schedule_R.thy
@@ -1034,6 +1034,7 @@ lemma threadSet_invs_no_cicd'_trivialT:
     "\<forall>tcb. tcbDomain tcb \<le> maxDomain \<longrightarrow> tcbDomain (F tcb) \<le> maxDomain"
     "\<forall>tcb. tcbPriority tcb \<le> maxPriority \<longrightarrow> tcbPriority (F tcb) \<le> maxPriority"
     "\<forall>tcb. tcbMCP tcb \<le> maxPriority \<longrightarrow> tcbMCP (F tcb) \<le> maxPriority"
+    "\<forall>tcb. tcbFlags tcb && ~~ tcbFlagMask = 0 \<longrightarrow> tcbFlags (F tcb) && ~~ tcbFlagMask = 0"
   shows
   "threadSet F t \<lbrace>invs_no_cicd'\<rbrace>"
   apply (simp add: invs_no_cicd'_def valid_state'_def)
